proof/garble/equivAda.ec
@@ -13,13 +13,192 @@ require import PreProof.
 require import Reduction.
 require import ReductionAda.
 
-lemma adaEq :
-  forall (ADV <: PrvIndSec.Adv_t{Red, DKCS.Dkc}),
-    equiv [
+equiv adaEq (ADV <: PrvIndSec.Adv_t{Red, RedAda, DKCS.Dkc}):
       DKCS.Game(DKCS.Dkc, Red(ADV)).main ~
       DKCS.GameAda(DKCS.Dkc, RedAda(ADV)).main
-      : (glob ADV){1} = (glob ADV){2} ==> res{1} = res{2}
-    ].
+        : (glob ADV){1} = (glob ADV){2} ==> res{1} = res{2}.
 proof strict.
+(** Preinitialization *)
+fun; seq 1 1: (={glob ADV, DKCS.Dkc.b} /\ Red.l{1} = RedAda.l{2} /\ 0 <= Red.l{1} < Cst.bound).
+  call (_: true ==> ={DKCS.Dkc.b} /\ Red.l{1} = RedAda.l{2} /\ 0 <= Red.l{1} < Cst.bound)=> //;
+  fun;
+    call (_: true ==> Red.l{1} = RedAda.l{2} /\ 0 <= Red.l{1} < Cst.bound); first by fun; rnd; skip; smt.
+    by call (_: true ==> ={DKCS.Dkc.b}); first by fun; eqobs_in.
+(** Experiment *)
+call (_: ={glob ADV, DKCS.Dkc.b} /\ Red.l{1} = RedAda.l{2} /\ 0 <= Red.l{1} < Cst.bound ==> ={res})=> //;
+fun; inline Red(ADV).gen_queries DKCS.GameAda(DKCS.Dkc, RedAda(ADV)).A.work.
+seq  2  2: (={glob ADV, glob DKCS.Dkc, info0, info} /\
+            Red.l{1} = RedAda.l{2} /\
+            0 <= Red.l{1} < Cst.bound);
+  first by wp; call (_: ={DKCS.Dkc.b} ==> ={glob DKCS.Dkc, res}); first by fun; wp; rnd; rnd.
+seq 1 1: (={glob ADV, glob DKCS.Dkc, info0} /\
+            Red.l{1} = RedAda.l{2} /\
+            Red.query{1} = RedAda.query{2} /\
+            0 <= Red.l{1} < Cst.bound);
+  first by call (_: true).
+case (!PrvIndSec.Scheme.queryValid Red.query){1}.
+  (** Invalid query *)
+  inline Red(ADV).get_challenge.
+  rcondf{1} 19; first by intros=> &m; wp; while true; do !(wp; call (_: true ==> true)=> //); wp; rnd.
+  rcondf{2} 11; first by intros=> &m; wp; rnd.
+  call (_: ={DKCS.Dkc.b})=> //; wp; rnd.
+    (* The rest is irrelevant *)
+    conseq* (_: ={DKCS.Dkc.b} ==> ={DKCS.Dkc.b})=> //.
+      wp; while{1} true (nquery - i){1};
+        first by intros=> &m z; wp; call (_: true ==> true); [by apply (DKCS.encryptL _); smt | skip; smt].
+      wp; call{1} (garble1L ADV).
+      by wp; rnd; skip; smt.
+(** Valid query *)
+inline Red(ADV).get_challenge.
+rcondt{1} 19; first by intros=> &m; wp; while true; do !(wp; call (_: true ==> true)=> //); wp; rnd; skip; smt.
+rcondt{2} 11; first by intros=> &m; wp; rnd; skip; smt.
+seq  0  0: (={glob ADV, glob DKCS.Dkc, info0} /\
+            Red.l{1} = RedAda.l{2} /\
+            0 <= Red.l{1} < Cst.bound /\
+            Red.query{1} = RedAda.query{2} /\
+            PrvIndSec.Scheme.queryValid Red.query{1});
+  first by skip; smt.
+seq 10 10: (={glob ADV, glob DKCS.Dkc} /\
+            Red.l{1} = RedAda.l{2} /\
+            Red.query{1} = RedAda.query{2} /\
+            Red.c{1} = RedAda.c{2} /\
+            Red.fc{1} = RedAda.fc{2} /\
+            Red.xc{1} = RedAda.xc{2} /\
+            Red.n{1} = RedAda.n{2} /\
+            Red.m{1} = RedAda.m{2} /\
+            Red.q{1} = RedAda.q{2} /\
+            Red.aa{1} = RedAda.aa{2} /\
+            Red.bb{1} = RedAda.bb{2} /\
+            Red.gg{1} = RedAda.gg{2} /\
+            Red.pp{1} = RedAda.pp{2} /\
+            Red.t{1} = RedAda.t{2} /\
+            Red.v{1} = RedAda.v{2} /\
+            Red.yy{1} = RedAda.yy{2} /\
+            Red.xx{1} = RedAda.xx{2} /\
+            Red.randG{1} = RedAda.randG{2} /\
+            Red.tau{1} = RedAda.tau{2} /\
+            length Red.v{1} = Red.n{1} + Red.q{1} /\
+            length Red.t{1} = Red.n{1} + Red.q{1} /\
+            0 <= Red.l{1} < Red.n{1} + Red.q{1}).
+  wp; rnd; wp; skip.
+    intros=> &1 &2 [[eqAdv [eqDkc eqInfo]] [eqL [[l_lb l_ub] [eqQuery validQuery]]]];
+      generalize validQuery; rewrite /PrvIndSec.Scheme.queryValid /PrvInd_Circuit.Scheme.queryValid;
+      intros=> Let; elim Let=> {Let} validCircuit1 [validCircuit2 H] {H}; generalize validCircuit1 validCircuit2;
+      rewrite /PrvInd_Circuit.Garble.functCorrect /functCorrect /validCircuit=> validCircuit1 validCircuit2;
+      generalize eqQuery l_ub l_lb eqL eqInfo eqDkc eqAdv;
+      progress=> //; smt. (* Well... that was fun *)
+seq  1  0: (={glob ADV, glob DKCS.Dkc} /\
+            Red.l{1} = RedAda.l{2} /\
+            Red.query{1} = RedAda.query{2} /\
+            Red.c{1} = RedAda.c{2} /\
+            Red.fc{1} = RedAda.fc{2} /\
+            Red.xc{1} = RedAda.xc{2} /\
+            Red.n{1} = RedAda.n{2} /\
+            Red.m{1} = RedAda.m{2} /\
+            Red.q{1} = RedAda.q{2} /\
+            Red.aa{1} = RedAda.aa{2} /\
+            Red.bb{1} = RedAda.bb{2} /\
+            Red.gg{1} = RedAda.gg{2} /\
+            Red.pp{1} = RedAda.pp{2} /\
+            Red.t{1} = RedAda.t{2} /\
+            Red.v{1} = RedAda.v{2} /\
+            Red.yy{1} = RedAda.yy{2} /\
+            Red.xx{1} = RedAda.xx{2} /\
+            Red.randG{1} = RedAda.randG{2} /\
+            Red.tau{1} = RedAda.tau{2} /\
+            Red.queries{1} = Array.empty /\
+            length Red.v{1} = Red.n{1} + Red.q{1} /\
+            length Red.t{1} = Red.n{1} + Red.q{1} /\
+            0 <= Red.l{1} < Red.n{1} + Red.q{1});
+  first by wp; skip; progress=> //;
+           rewrite /Array.create empty_unique // ?init_length //.
+inline Red(ADV).garble1 Red(ADV).garble2 RedAda(ADV,DKCS.Dkc).garble Red(ADV).get_challenge.
+seq  5  5: (={glob ADV, glob DKCS.Dkc} /\
+            Red.l{1} = RedAda.l{2} /\
+            Red.query{1} = RedAda.query{2} /\
+            Red.c{1} = RedAda.c{2} /\
+            Red.fc{1} = RedAda.fc{2} /\
+            Red.xc{1} = RedAda.xc{2} /\
+            Red.n{1} = RedAda.n{2} /\
+            Red.m{1} = RedAda.m{2} /\
+            Red.q{1} = RedAda.q{2} /\
+            Red.aa{1} = RedAda.aa{2} /\
+            Red.bb{1} = RedAda.bb{2} /\
+            Red.gg{1} = RedAda.gg{2} /\
+            Red.pp{1} = RedAda.pp{2} /\
+            Red.t{1} = RedAda.t{2} /\
+            Red.v{1} = RedAda.v{2} /\
+            Red.yy{1} = RedAda.yy{2} /\
+            Red.xx{1} = RedAda.xx{2} /\
+            Red.randG{1} = RedAda.randG{2} /\
+            Red.tau{1} = RedAda.tau{2} /\
+            Red.queries{1} = Array.empty /\
+            Red.i{1} = RedAda.i{2} /\
+            Red.v{1} = RedAda.v{2} /\
+            Red.t{1} = RedAda.t{2} /\
+            Red.g{1} = RedAda.g{2} /\
+            length Red.v{1} = Red.n{1} + Red.q{1} /\
+            length Red.t{1} = Red.n{1} + Red.q{1} /\
+            0 <= Red.l{1} < Red.n{1} + Red.q{1}).
+  wp; while (Red.i{1} = RedAda.i{2} /\
+             Red.n{1} = RedAda.n{2} /\
+             Red.q{1} = RedAda.q{2} /\
+             Red.fc{1} = RedAda.fc{2} /\
+             Red.xc{1} = RedAda.xc{2} /\
+             length Red.v{1} = length RedAda.v{2} /\
+             length Red.t{1} = length RedAda.t{2} /\
+             length Red.v{1} = Red.n{1} + Red.q{1} /\
+             length Red.t{1} = Red.n{1} + Red.q{1} /\
+             (forall j, 0 <= j < Red.n{1} + Red.q{1} =>
+               Red.v.[j]{1} = RedAda.v.[j]{2}) /\
+             (forall j, 0 <= j < Red.n{1} + Red.q{1} =>
+               Red.t.[j]{1} = RedAda.t.[j]{2})).
+    wp; skip; progress=> //; first 4 smt.
+      by case (j = RedAda.i){2}; [smt | intros=> neq; rewrite 2?set_get // /=; smt].
+      by case (j = RedAda.i){2}; smt.
+  while (Red.i{1} = RedAda.i{2} /\
+         Red.n{1} = RedAda.n{2} /\
+         Red.m{1} = RedAda.m{2} /\
+         Red.q{1} = RedAda.q{2} /\
+         Red.fc{1} = RedAda.fc{2} /\
+         Red.xc{1} = RedAda.xc{2} /\
+         length Red.v{1} = length RedAda.v{2} /\
+         length Red.t{1} = length RedAda.t{2} /\
+         length Red.v{1} = Red.n{1} + Red.q{1} /\
+         length Red.t{1} = Red.n{1} + Red.q{1} /\
+         (forall j, 0 <= j < Red.n{1} + Red.q{1} =>
+           Red.v.[j]{1} = RedAda.v.[j]{2}) /\
+         (forall j, 0 <= j < Red.n{1} + Red.q{1} =>
+           Red.t.[j]{1} = RedAda.t.[j]{2})).
+    wp; rnd; wp; skip; progress=> //; first 4 smt.
+      by case (j = RedAda.i){2}; [smt | intros=> neq; rewrite 2?set_get // /=; smt].
+      by case (j = RedAda.i){2}; smt.
+  wp; skip; progress=> //.
+    by rewrite H9.
+    by rewrite H10.
+    apply extensionality; rewrite /Array.(==); progress=> //.
+      smt.
+      by case (i0 = RedAda.l){2}; [smt | intros=> neq; rewrite 2?set_get // /=; smt].
+    by apply extensionality; rewrite /Array.(==); progress=> //; smt.
+    by apply extensionality; rewrite /Array.(==); progress=> //; smt.
+    apply extensionality; rewrite /Array.(==); progress=> //.
+      smt.
+      by case (i0 = RedAda.l){2}; [smt | intros=> neq; rewrite 2?set_get // /=; smt].
+    smt.
+
+  (* Loop manipulation goes here *)
+
+  (*right*)
+  inline DKCS.Dkc.get_challenge.
+  inline RedAda(ADV, DKCS.Dkc).garble.
+
+  (*left*)
+  inline DKCS.Game(DKCS.Dkc, Red(ADV)).work.
+  inline Red(ADV).gen_queries.
+  inline Red(ADV).get_challenge.
+  inline Red(ADV).garble1.
+  inline Red(ADV).garble2.
+
+
   admit.
-save.
+qed.
